fairness/fuel_termination.v
@@ -1,12 +1,16 @@
 From stdpp Require Import option.
 From Paco Require Import pacotac.
-From trillium.fairness Require Export fairness fair_termination fuel.
+From trillium.fairness Require Export fairness fair_termination fuel traces_match.
 
 Definition auxtrace_fairly_terminating {Λ} {Mdl : FairModel}
-           {LM : LiveModel (locale Λ) Mdl} (auxtr : auxtrace (LM := LM)) :=
+           {LM : LiveModel (locale Λ) Mdl} (auxtr : auxtrace (M := LM)) :=
   auxtrace_valid (LM:=LM) auxtr →
-  (∀ ρ, fair_aux ρ auxtr) →
+  (∀ ρ, fair_aux ρ auxtr (LM := LM)) →
   terminating_trace auxtr.
+
+Definition lm_valid_state_evolution_fairness 
+  `{LM:LiveModel (locale Λ) M} `{EqDecision (locale Λ)} := 
+  valid_state_evolution_fairness (M := LM) lm_valid_evolution_step.
 
 Theorem continued_simulation_fair_termination
         `{FairTerminatingModel FM} `(LM:LiveModel (locale Λ) FM) `{Countable (locale Λ)}
@@ -18,7 +22,7 @@ Theorem continued_simulation_fair_termination
      ξ ex atr -> live_tids (LM:=LM) (trace_last ex) (trace_last atr)) ->
   (* The relation must capture that the traces evolve fairly *)
   (forall (ex: execution_trace Λ) (atr: auxiliary_trace LM),
-     ξ ex atr -> valid_state_evolution_fairness ex atr) →
+     ξ ex atr -> lm_valid_state_evolution_fairness ex atr) →
   continued_simulation
     ξ ({tr[trfirst extr]}) ({tr[initial_ls a1 r1]}) →
   extrace_fairly_terminating extr.
@@ -36,17 +40,28 @@ Proof.
     Unshelve.
     - done.
     - eapply from_trace_preserves_validity; eauto; first econstructor. }
-  assert (∃ (auxtr : auxtrace (LM := LM)), exaux_traces_match extr auxtr)
+  assert (∃ (auxtr : auxtrace (M := LM)), 
+             exaux_traces_match 
+               (* (live_tids (LM := LM)) *)
+               (fun c (δ: mstate LM) => live_tids c δ (LM := LM))
+
+               (labels_match (LM := LM)) extr auxtr)
     as [auxtr Hmatch].
   { exists (to_trace (initial_ls a1 r1) iatr).
-    eapply (valid_inf_system_trace_implies_traces_match
+    unshelve eapply (valid_inf_system_trace_implies_traces_match
+              (lm_valid_evolution_step (LM := LM))
+              live_tids
+              labels_match
+              ltac:(idtac)
+              ltac:(idtac)
               (continued_simulation ξ)); eauto.
+    1, 2: intros ?????? V; by apply V. 
     - intros ? ? ?%continued_simulation_rel. by apply Hlive.
     - intros ? ? ?%continued_simulation_rel. by apply Hvalid.
     - by apply from_trace_spec.
     - by apply to_trace_spec. }
   intros Hfair.
-  assert (auxtrace_valid auxtr) as Hstutter.
+  assert (auxtrace_valid auxtr (LM := LM)) as Hstutter.
   { by eapply exaux_preserves_validity. }
   apply can_destutter_auxtr in Hstutter.
   destruct Hstutter as [mtr Hupto].
