fairness/traces_match.v
@@ -1,0 +1,108 @@
+From iris.proofmode Require Import tactics.
+From trillium Require Import language.
+From trillium.fairness Require Import inftraces fairness. 
+
+
+Section TracesMatch.
+  Context `{Λ: language}.
+  Context `{M: Model}. 
+
+  Definition auxtrace := trace (mstate M) (mlabel M).
+
+  Context (evolution_pred: cfg Λ -> olocale Λ → cfg Λ → 
+                           M → mlabel M → M -> Prop). 
+
+  Context (state_rel: cfg Λ -> mstate M -> Prop).
+  Context (lbl_rel: olocale Λ -> mlabel M -> Prop).
+  Hypothesis (LBL_REL_EV: forall c1 oζ c2 δ1 ℓ δ2,
+                 evolution_pred c1 oζ c2 δ1 ℓ δ2 ->
+                 lbl_rel oζ ℓ).
+  Hypothesis (STEP_EV: forall c1 oζ c2 δ1 ℓ δ2,
+                 evolution_pred c1 oζ c2 δ1 ℓ δ2 ->
+                 mtrans δ1 ℓ δ2).
+
+  Definition exaux_traces_match:
+    extrace Λ → auxtrace → Prop :=
+    traces_match lbl_rel
+      state_rel
+      locale_step
+      (@mtrans M).
+
+  Lemma valid_inf_system_trace_implies_traces_match_strong'
+        (φ : execution_trace Λ -> auxiliary_trace M -> Prop)
+        ex atr iex iatr progtr (auxtr : auxtrace):
+    (forall (ex: execution_trace Λ) (atr: auxiliary_trace M),
+        φ ex atr -> state_rel (trace_last ex) (trace_last atr)) ->
+    (forall (ex: execution_trace Λ) (oζ: olocale Λ) (c: cfg Λ) 
+       (atr: auxiliary_trace M) (ℓ: mlabel M) (δ: mstate M),
+        φ (ex :tr[ oζ ]: c) (atr :tr[ ℓ ]: δ) -> 
+        evolution_pred (trace_last ex) oζ c (trace_last atr) ℓ δ) ->
+    exec_trace_match ex iex progtr ->
+    exec_trace_match atr iatr auxtr ->
+    valid_inf_system_trace φ ex atr iex iatr ->
+    traces_match lbl_rel
+                 state_rel
+                 locale_step
+                 (@mtrans M) progtr auxtr.
+  Proof.
+    intros Hφ1 Hφ2.
+    revert ex atr iex iatr auxtr progtr. cofix IH.
+    intros ex atr iex iatr auxtr progtr Hem Ham Hval.
+    inversion Hval as [?? Hphi |ex' atr' c [? σ'] δ' iex' iatr' oζ ℓ Hphi [=] ? Hinf]; simplify_eq.
+    - inversion Hem; inversion Ham. econstructor; eauto.
+      pose proof (Hφ1 ex atr Hphi).
+      by simplify_eq. 
+    - inversion Hem; inversion Ham. subst.
+      pose proof (valid_inf_system_trace_inv _ _ _ _ _ Hinf) as Hphi'.
+      specialize (Hφ2 _ _ _ _ _ _ Hphi') as STEP.
+      econstructor.
+      + eapply LBL_REL_EV; eauto.
+      + eauto.
+      + match goal with
+        | [H: exec_trace_match _ iex' _ |- _] => inversion H; clear H; simplify_eq
+        end; done.
+      + match goal with
+        | [H: exec_trace_match _ iatr' _ |- _] => inversion H; clear H; simplify_eq
+        end; eapply STEP_EV; eauto.
+      + eapply IH; eauto.
+  Qed.
+
+
+  Definition valid_state_evolution_fairness
+             (extr : execution_trace Λ) (auxtr : auxiliary_trace M) :=
+    match extr, auxtr with
+    | (extr :tr[oζ]: (es, σ)), auxtr :tr[ℓ]: δ =>
+        evolution_pred (trace_last extr) oζ (es, σ) (trace_last auxtr) ℓ δ
+    | _, _ => True
+    end.
+
+  Definition valid_lift_fairness
+             (φ: execution_trace Λ -> auxiliary_trace M -> Prop)
+             (extr : execution_trace Λ) (auxtr : auxiliary_trace M) :=
+    valid_state_evolution_fairness extr auxtr ∧ φ extr auxtr.
+
+  (* TODO: this should already be covered by .._strong' lemma above *)
+  (* Lemma valid_inf_system_trace_implies_traces_match_strong *)
+
+  Lemma valid_inf_system_trace_implies_traces_match
+        (φ : execution_trace Λ -> auxiliary_trace M -> Prop)
+        (* (ψ : _ → _ → Prop) *)
+        ex atr iex iatr progtr (auxtr : auxtrace):
+    (forall (ex: execution_trace Λ) (atr: auxiliary_trace M),
+        φ ex atr -> state_rel (trace_last ex) (trace_last atr)) ->
+    (forall (ex: execution_trace Λ) (atr: auxiliary_trace M),
+        φ ex atr -> valid_state_evolution_fairness ex atr) ->
+    exec_trace_match ex iex progtr ->
+    exec_trace_match atr iatr auxtr ->
+    valid_inf_system_trace φ ex atr iex iatr ->
+    traces_match lbl_rel
+                 state_rel
+                 locale_step
+                 (@mtrans M) progtr auxtr. 
+  Proof.
+    intros. eapply valid_inf_system_trace_implies_traces_match_strong'; eauto.
+    intros. apply H0 in H4. red in H4. by destruct c. 
+  Qed. 
+
+
+End TracesMatch.
